unclear how to prove unique_mGive_footprint
even after changing it to quantifying only over one trace instead
of two

bedrock2/src/bedrock2/StateMachineBasedExtSpec_wp.v
@@ -19,16 +19,52 @@ Section WithMem.
             (mem -> list word -> state -> Prop) ->
             Prop).
 
-  Fixpoint trace_leads_to_state_satisfying(t: trace)(post: state -> Prop): Prop :=
+  Fixpoint apply_trace(s0: state)(t: trace)(post: state -> Prop): Prop :=
     match t with
-    | nil => forall s, is_initial_state s -> post s
+    | nil => post s0
     | cons ((mGive, action, args), (mReceive, rets)) t' =>
-        trace_leads_to_state_satisfying t' (fun s =>
-          step s mGive action args (fun mReceive' rets' s' =>
+        apply_trace s0 t' (fun s1 =>
+          step s1 mGive action args (fun mReceive' rets' s2 =>
             mReceive' = mReceive ->
             rets' = rets ->
-            post s'))
+            post s2))
     end.
+
+  Definition trace_leads_to_state_satisfying(t: trace)(post: state -> Prop): Prop :=
+    forall s, is_initial_state s -> apply_trace s t post.
+
+  Lemma apply_trace_app: forall t1 t2 s post,
+      (* note the reversed order: elements at the head of the trace happened last! *)
+      apply_trace s t2 (fun s' => apply_trace s' t1 post) ->
+      apply_trace s (List.app t1 t2) post.
+  Proof.
+    induction t1; simpl; intros.
+    - assumption.
+    - destruct a as (((mGive & action) & args) & (mReceive & rets)).
+      eapply IHt1. exact H.
+  Qed.
+
+  Lemma invert_apply_trace_app: forall t1 t2 s post,
+      apply_trace s (List.app t1 t2) post ->
+      apply_trace s t2 (fun s' => apply_trace s' t1 post).
+  Proof.
+    induction t1; simpl; intros.
+    - assumption.
+    - destruct a as (((mGive & action) & args) & (mReceive & rets)).
+      eapply IHt1. exact H.
+  Qed.
+
+  Lemma apply_trace_snoc: forall t mGive action args mReceive rets s post,
+      step s mGive action args (fun mReceive' rets' s' =>
+        mReceive' = mReceive -> rets' = rets -> apply_trace s' t post) ->
+      apply_trace s (List.app t (cons ((mGive, action, args), (mReceive, rets)) nil)) post.
+  Proof. intros. eapply apply_trace_app. simpl. assumption. Qed.
+
+  Lemma invert_apply_trace_snoc: forall t mGive action args mRcv rets s post,
+      apply_trace s (List.app t (cons ((mGive, action, args), (mRcv, rets)) nil)) post ->
+      step s mGive action args (fun mRcv' rets' s' =>
+        mRcv' = mRcv -> rets' = rets -> apply_trace s' t post).
+  Proof. intros. eapply invert_apply_trace_app in H. simpl in H. assumption. Qed.
 
   Hypothesis weaken_step: forall s mGive action args
                                  (post1 post2: mem -> list word -> state -> Prop),
@@ -36,10 +72,10 @@ Section WithMem.
       (forall mReceive rets s', post1 mReceive rets s' -> post2 mReceive rets s') ->
       step s mGive action args post2.
 
-  Lemma weaken_trace_leads_to_state_satisfying: forall t (post1 post2: state -> Prop),
-      trace_leads_to_state_satisfying t post1 ->
+  Lemma weaken_apply_trace: forall t s (post1 post2: state -> Prop),
+      apply_trace s t post1 ->
       (forall s, post1 s -> post2 s) ->
-      trace_leads_to_state_satisfying t post2.
+      apply_trace s t post2.
   Proof.
     induction t; simpl; intros.
     - eauto.
@@ -47,6 +83,52 @@ Section WithMem.
       eapply IHt. 1: exact H. cbv beta.
       intros. eapply weaken_step. 1: eassumption. cbv beta. eauto.
   Qed.
+
+  Lemma apply_trace_induction: forall s0 inv,
+      inv s0 ->
+      (forall s, inv s -> forall mGive action args,
+            step s mGive action args (fun _ _ s' => inv s')) ->
+      forall t, apply_trace s0 t inv.
+  Proof.
+    induction t; simpl; intros.
+    - assumption.
+    - destruct a as (((mGive & action) & args) & (mReceive & rets)).
+      eapply weaken_apply_trace. 1: exact IHt. eauto.
+  Qed.
+
+  Lemma apply_snoc_trace_induction: forall P: state -> trace -> (state -> Prop) -> Prop,
+      (forall s (post: state -> Prop), post s -> P s nil post) ->
+      (forall t s mGive action args mReceive rets mid post,
+          step s mGive action args mid ->
+          (forall s', mid mReceive rets s' -> apply_trace s' t post /\ P s' t post) ->
+          P s (List.app t (cons ((mGive, action, args), (mReceive, rets)) nil)) post) ->
+      forall t s post, apply_trace s t post -> P s t post.
+  Proof.
+    intros until t.
+    set (n := List.length t).
+    pose proof (eq_refl: n = List.length t) as HL. clearbody n.
+    revert t HL. induction n; intros.
+    - destruct t. 2: discriminate HL. simpl in H. eauto.
+    - pose proof (List.firstn_skipn n t) as Hsplit.
+      pose proof (List.length_skipn n t) as HL2.
+      rewrite <- HL in HL2. rewrite Nat.sub_succ_l in HL2 by reflexivity.
+      rewrite Nat.sub_diag in HL2.
+      destruct (List.skipn n t) as [ |h' t']. 1: discriminate HL2.
+      destruct t'. 2: discriminate HL2.
+      clear HL2. set (tl := List.firstn n t) in *. clearbody tl. subst t.
+      rewrite List.app_length in HL. simpl in HL. rewrite Nat.add_comm in HL.
+      eapply Nat.succ_inj in HL. specialize IHn with (1 := HL).
+      destruct h' as (((mGive & action) & args) & (mReceive & rets)).
+      eapply invert_apply_trace_snoc in H1.
+      eapply H0. 1: exact H1. cbv beta.
+      intros * HA. clear -HA IHn. eauto.
+  Qed.
+
+  Lemma weaken_trace_leads_to_state_satisfying: forall t (post1 post2: state -> Prop),
+      trace_leads_to_state_satisfying t post1 ->
+      (forall s, post1 s -> post2 s) ->
+      trace_leads_to_state_satisfying t post2.
+  Proof. unfold trace_leads_to_state_satisfying. eauto using weaken_apply_trace. Qed.
 
   Definition ext_spec: ExtSpec :=
     fun (t: trace)(mGive: mem)(action: String.string)(args: list word)
@@ -57,7 +139,7 @@ Section WithMem.
   Lemma ext_spec_ok: ext_spec.ok ext_spec.
   Proof.
     unfold ext_spec. constructor.
-    - intros. (* ?? *) admit.
+    - unfold trace_leads_to_state_satisfying. intros. (* ?? *) admit.
     - unfold Morphisms.Proper, Morphisms.respectful, Morphisms.pointwise_relation,
         Basics.impl.
       intros. eapply weaken_trace_leads_to_state_satisfying. 1: eassumption.
